Test/civl/samples/reserve2.bpl
@@ -1,0 +1,265 @@
+// RUN: %parallel-boogie "%s" > "%t"
+// RUN: %diff "%s.expect" "%t"
+
+/*
+This example models a memory allocator based on count of free cells (freeSpace) and an
+array that keeps tracks of the allocation status of each cell (isFree). To allocate
+a cell, freeSpace is decremented atomically, blocking to ensure that freeSpace does not
+go below zero. If the decrement succeeds, then a scan of isFree is performed to find a
+free cell. The goal of the verification is to prove that this scan will succeed. The
+main challenge in the proof is to reason about cardinality of constructed sets.
+
+The layer transformations are as follows:
+1 -> 2: transform isFree array into the finite set isFreeSet enabling cardinality reasoning
+2 -> 3: use cardinality reasoning to transform freeSpace into the bijection allocMap
+
+The verification goal is discharged at layer 3.
+*/
+
+datatype Bijection {
+  Bijection(tidToPtr: Map Tid int, ptrToTid: Map int Tid)
+}
+
+function {:inline} BijectionInvariant(allocMap: Bijection): bool {
+    (forall tid: Tid ::
+        Map_Contains(allocMap->tidToPtr, tid) ==>
+            (var x := Map_At(allocMap->tidToPtr, tid); Map_Contains(allocMap->ptrToTid, x) && Map_At(allocMap->ptrToTid, x) == tid))
+    &&
+    (forall ptr: int ::
+        Map_Contains(allocMap->ptrToTid, ptr) ==>
+            (var x := Map_At(allocMap->ptrToTid, ptr); Map_Contains(allocMap->tidToPtr, x) && Map_At(allocMap->tidToPtr, x) == ptr))
+}
+
+type {:linear "tid"} Tid = int;
+
+const memLo: int;
+const memHi: int;
+axiom 0 < memLo && memLo <= memHi;
+function {:inline} memAddr(i: int) returns (bool) { memLo <= i && i < memHi }
+
+var {:layer 0,1} isFree: [int]bool;
+var {:layer 1,3} isFreeSet: Set int;
+var {:layer 0,2} freeSpace: int;
+var {:layer 2,3} allocMap: Bijection;
+
+yield procedure {:layer 3} Malloc({:linear "tid"} tid: Tid)
+preserves call YieldInvariant#1();
+preserves call YieldInvariant#2(tid, false);
+preserves call YieldInvariant#3(tid, false, memLo);
+{
+    var i: int;
+    var spaceFound: bool;
+
+    call DecrementFreeSpace#2(tid);
+    i := memLo;
+    while (i < memHi)
+    invariant {:yields} true;
+    invariant {:layer 1, 2} memLo <= i && i <= memHi;
+    invariant {:layer 3} memAddr(i);
+    invariant call YieldInvariant#1();
+    invariant call YieldInvariant#2(tid, true);
+    invariant call YieldInvariant#3(tid, true, i);
+    {
+        call spaceFound := AllocIfPtrFree#2(tid, i);
+        if (spaceFound)
+        {
+            return;
+        }
+        i := i + 1;
+    }
+    call Unreachable(); // verification goal
+}
+
+yield procedure {:layer 3} Collect()
+preserves call YieldInvariant#1();
+{
+    var ptr: int;
+
+    while (*)
+    invariant {:yields} true;
+    invariant call YieldInvariant#1();
+    {
+        call ptr := Reclaim#2();
+    }
+}
+
+action {:layer 2,3} Alloc(tid: Tid, ptr: int)
+modifies allocMap;
+{
+    var tid': Tid;
+    var ptr': int;
+    assert Map_Contains(allocMap->tidToPtr, tid);
+    if (Map_Contains(allocMap->ptrToTid, ptr)) {
+        // swap
+        tid' := Map_At(allocMap->ptrToTid, ptr);
+        ptr' := Map_At(allocMap->tidToPtr, tid);
+        allocMap := Bijection(Map_Swap(allocMap->tidToPtr, tid, tid'), Map_Swap(allocMap->ptrToTid, ptr, ptr'));
+    }
+    // alloc
+    ptr' := Map_At(allocMap->tidToPtr, tid);
+    allocMap := Bijection(Map_Remove(allocMap->tidToPtr, tid), Map_Remove(allocMap->ptrToTid, ptr'));
+}
+
+action {:layer 2,3} PreAlloc({:linear "tid"} tid: Tid, set: Set int)
+modifies allocMap;
+{
+    var ptr: int;
+    assert set != Set_Empty();
+    ptr := Set_Choose(set);
+    allocMap := Bijection(Map_Update(allocMap->tidToPtr, tid, ptr), Map_Update(allocMap->ptrToTid, ptr, tid));
+}
+
+atomic action {:layer 3} AtomicDecrementFreeSpace#2({:linear "tid"} tid: Tid)
+modifies allocMap;
+{
+    var set: Set int;
+    set := Set_Difference(isFreeSet, allocMap->ptrToTid->dom);
+    assume set != Set_Empty();
+    call PreAlloc(tid, set);
+}
+yield procedure {:layer 2} DecrementFreeSpace#2({:linear "tid"} tid: Tid)
+refines AtomicDecrementFreeSpace#2;
+preserves call YieldInvariant#1();
+requires call YieldInvariant#2(tid, false);
+ensures call YieldInvariant#2(tid, true);
+{
+    var set: Set int;
+    call DecrementFreeSpace#0(tid);
+    call PreAlloc(tid, Set_Difference(isFreeSet, allocMap->ptrToTid->dom));
+}
+
+atomic action {:layer 1,2} AtomicDecrementFreeSpace#0({:linear "tid"} tid: Tid)
+modifies freeSpace;
+{
+    assume 0 < freeSpace;
+    freeSpace := freeSpace - 1;
+}
+yield procedure {:layer 0} DecrementFreeSpace#0({:linear "tid"} tid: Tid);
+refines AtomicDecrementFreeSpace#0;
+
+atomic action {:layer 3} AtomicAllocIfPtrFree#2({:linear "tid"} tid: Tid, ptr: int) returns (spaceFound:bool)
+modifies isFreeSet, allocMap;
+{
+    assert memAddr(ptr);
+    spaceFound := Set_Contains(isFreeSet, ptr);
+    if (spaceFound) {
+        isFreeSet := Set_Remove(isFreeSet, ptr);
+        call Alloc(tid, ptr);
+    }
+}
+yield procedure {:layer 2} AllocIfPtrFree#2({:linear "tid"} tid: Tid, ptr: int) returns (spaceFound:bool)
+refines AtomicAllocIfPtrFree#2;
+preserves call YieldInvariant#1();
+requires call YieldInvariant#2(tid, true);
+ensures call YieldInvariant#2(tid, !spaceFound);
+{
+    call spaceFound := AllocIfPtrFree#1(tid, ptr);
+    if (spaceFound) {
+        call Alloc(tid, ptr);
+    }
+}
+
+atomic action {:layer 2} AtomicAllocIfPtrFree#1({:linear "tid"} tid: Tid, ptr: int) returns (spaceFound:bool)
+modifies isFreeSet;
+{
+    assert memAddr(ptr);
+    spaceFound := Set_Contains(isFreeSet, ptr);
+    if (spaceFound) {
+        isFreeSet := Set_Remove(isFreeSet, ptr);
+    }
+}
+yield procedure {:layer 1} AllocIfPtrFree#1({:linear "tid"} tid: Tid, ptr: int) returns (spaceFound:bool)
+refines AtomicAllocIfPtrFree#1;
+preserves call YieldInvariant#1();
+{
+    call spaceFound := AllocIfPtrFree#0(tid, ptr);
+    if (spaceFound) {
+        call IsFreeSetRemove(ptr);
+    }
+}
+
+atomic action {:layer 1} AtomicAllocIfPtrFree#0({:linear "tid"} tid: Tid, ptr: int) returns (spaceFound:bool)
+modifies isFree;
+{
+    assert memAddr(ptr);
+    spaceFound := isFree[ptr];
+    if (spaceFound) {
+        isFree[ptr] := false;
+    }
+}
+yield procedure {:layer 0} AllocIfPtrFree#0({:linear "tid"} tid: Tid, ptr: int) returns (spaceFound:bool);
+refines AtomicAllocIfPtrFree#0;
+
+atomic action {:layer 3} AtomicReclaim#2() returns (ptr: int)
+modifies isFreeSet;
+{
+    assume memAddr(ptr) && !Set_Contains(isFreeSet, ptr);
+    isFreeSet := Set_Add(isFreeSet, ptr);
+}
+yield procedure {:layer 2} Reclaim#2() returns (ptr: int)
+refines AtomicReclaim#2;
+preserves call YieldInvariant#1();
+{
+    call ptr := Reclaim#1();
+}
+
+action {:layer 1,2} IsFreeSetAdd(ptr: int)
+modifies isFreeSet;
+{
+    isFreeSet := Set_Add(isFreeSet, ptr);
+}
+
+action {:layer 1,2} IsFreeSetRemove(ptr: int)
+modifies isFreeSet;
+{
+    isFreeSet := Set_Remove(isFreeSet, ptr);
+}
+
+atomic action {:layer 2} AtomicReclaim#1() returns (ptr: int)
+modifies freeSpace, isFreeSet;
+{
+    assume memAddr(ptr) && !Set_Contains(isFreeSet, ptr);
+    freeSpace := freeSpace + 1;
+    isFreeSet := Set_Add(isFreeSet, ptr);
+}
+yield procedure {:layer 1} Reclaim#1() returns (ptr: int)
+refines AtomicReclaim#1;
+preserves call YieldInvariant#1();
+{
+    call ptr := Reclaim#0();
+    call IsFreeSetAdd(ptr);
+}
+
+atomic action {:layer 1} AtomicReclaim#0() returns (ptr: int)
+modifies freeSpace, isFree;
+{
+    assume memAddr(ptr) && !isFree[ptr];
+    freeSpace := freeSpace + 1;
+    isFree[ptr] := true;
+}
+yield procedure {:layer 0} Reclaim#0() returns (ptr: int);
+refines AtomicReclaim#0;
+
+left action {:layer 1,3} AtomicUnreachable()
+{
+    assert false;
+}
+yield procedure {:layer 0} Unreachable();
+refines AtomicUnreachable;
+
+yield invariant {:layer 1} YieldInvariant#1();
+invariant (forall y: int :: Set_Contains(isFreeSet, y) <==> memAddr(y) && isFree[y]);
+
+yield invariant {:layer 2} YieldInvariant#2({:linear "tid"} tid: Tid, status: bool);
+invariant Map_Contains(allocMap->tidToPtr, tid) == status;
+invariant 0 <= freeSpace;
+invariant freeSpace == Set_Size(Set_Difference(isFreeSet, allocMap->ptrToTid->dom));
+invariant Set_IsSubset(allocMap->ptrToTid->dom, isFreeSet);
+invariant BijectionInvariant(allocMap);
+
+yield invariant {:layer 3} YieldInvariant#3({:linear "tid"} tid: Tid, status: bool, i: int);
+invariant Map_Contains(allocMap->tidToPtr, tid) == status;
+invariant Set_IsSubset(allocMap->ptrToTid->dom, isFreeSet);
+invariant BijectionInvariant(allocMap);
+invariant (forall y: int :: Set_Contains(isFreeSet, y) ==> memAddr(y));
+invariant Map_Contains(allocMap->tidToPtr, tid) ==> i <= Map_At(allocMap->tidToPtr, tid);
